p256: use complete point addition and doubling formulas

code/ecdsap256/Hacl.Impl.P256.DH.fst
@@ -19,51 +19,46 @@ module BSeq = Lib.ByteSequence
 
 let ecp256dh_i public_key private_key =
   push_frame ();
-  let pk = create_point () in
-  point_mul_g_bytes pk private_key;
-  let flag = is_point_at_inf pk in
-  aff_point_store public_key (sub pk 0ul 8ul);
+  let pk = create_aff_point () in
+  let flag = point_mul_g_bytes pk private_key in
+  aff_point_store public_key pk;
   pop_frame ();
-
   Hacl.Bignum.Base.unsafe_bool_of_limb0 flag
 
 
 inline_for_extraction noextract
 val ecp256dh_r_:
     is_pk_valid:bool
-  -> ss:point
+  -> ss:aff_point
   -> pk:point
   -> private_key:lbuffer uint8 32ul ->
   Stack uint64
   (requires fun h ->
     live h ss /\ live h pk /\ live h private_key /\
     disjoint ss pk /\ disjoint ss private_key /\ disjoint pk private_key /\
-    (is_pk_valid ==> point_inv h pk) /\ as_point_nat h ss = (0, 0, 0))
+    (is_pk_valid ==> point_inv h pk) /\ as_aff_point_nat h ss = (0, 0))
   (ensures fun  h0 flag h1 -> modifies (loc ss) h0 h1 /\
-    as_point_nat h1 ss ==
-    (if is_pk_valid then
-      S.norm_jacob_point (S.point_mul 
-        (BSeq.nat_from_bytes_be (as_seq h0 private_key)) (as_point_nat h0 pk))
-    else (0, 0, 0)) /\
+    (let sk_nat = BSeq.nat_from_bytes_be (as_seq h0 private_key) in
+    as_aff_point_nat h1 ss ==
+    (if is_pk_valid then S.to_aff_point (S.point_mul sk_nat (as_point_nat h0 pk)) else (0, 0)) /\
     v flag ==
-    (if is_pk_valid then (if S.is_point_at_inf (as_point_nat h1 ss) then ones_v U64 else 0)
-    else ones_v U64))
+    (if is_pk_valid then (if S.is_point_at_inf (S.point_mul sk_nat (as_point_nat h0 pk))
+     then ones_v U64 else 0) else ones_v U64)))
 
 let ecp256dh_r_ is_pk_valid ss pk private_key =
-  if is_pk_valid then begin
-    point_mul_bytes ss pk private_key;
-    is_point_at_inf ss end
+  if is_pk_valid then
+    point_mul_bytes ss pk private_key
   else
     ones U64 SEC
 
 
 let ecp256dh_r shared_secret their_pubkey private_key =
   push_frame ();
-  let ss = create_point () in
   let pk = create_point () in
   let is_pk_valid = load_point_vartime pk their_pubkey in
-  let flag = ecp256dh_r_ is_pk_valid ss pk private_key in
-  aff_point_store shared_secret (sub ss 0ul 8ul);
-  pop_frame ();
 
+  let ss = create_aff_point () in
+  let flag = ecp256dh_r_ is_pk_valid ss pk private_key in
+  aff_point_store shared_secret ss;
+  pop_frame ();
   Hacl.Bignum.Base.unsafe_bool_of_limb0 flag
