code/ecdsap256/Hacl.Impl.P256.PointAdd.fst
@@ -17,218 +17,271 @@ module SM = Hacl.Spec.P256.Montgomery
 #reset-options "--z3rlimit 50 --fuel 0 --ifuel 0"
 
 inline_for_extraction noextract
-val point_add_u12_s12: u1:felem -> u2:felem -> s1:felem -> s2:felem -> p:point -> q:point ->
-  Stack unit
+val point_add_1 (t0 t1 t2 t3 t4:felem) (p q:point) : Stack unit
   (requires fun h ->
-    live h u1 /\ live h u2 /\ live h s1 /\ live h s2 /\ live h p /\ live h q /\
-    LowStar.Monotonic.Buffer.all_disjoint [loc p; loc q; loc u1; loc u2; loc s1; loc s2] /\
-    point_inv h p /\ point_inv h q)
-  (ensures fun h0 _ h1 ->
-    modifies (loc u1 |+| loc u2 |+| loc s1 |+| loc s2) h0 h1 /\
-    as_nat h1 u1 < S.prime /\ as_nat h1 u2 < S.prime /\
-    as_nat h1 s1 < S.prime /\ as_nat h1 s2 < S.prime /\
-    (let px, py, pz = from_mont_point (as_point_nat h0 p) in
-    let qx, qy, qz = from_mont_point (as_point_nat h0 q) in
-    let z2z2 = S.fmul qz qz in
-    let z1z1 = S.fmul pz pz in
-    fmont_as_nat h1 u1 == S.fmul px z2z2 /\
-    fmont_as_nat h1 u2 == S.fmul qx z1z1 /\
-    fmont_as_nat h1 s1 == S.fmul (S.fmul py qz) z2z2 /\
-    fmont_as_nat h1 s2 == S.fmul (S.fmul qy pz) z1z1))
-
-let point_add_u12_s12 u1 u2 s1 s2 p q =
-  let px = getx p in
-  let py = gety p in
-  let pz = getz p in
-
-  let qx = getx q in
-  let qy = gety q in
-  let qz = getz q in
-
-  let h0 = ST.get () in
-  fsqr s1 qz;           // s1 = z2z2 = qz * qz
-  fsqr s2 pz;           // s2 = z1z1 = pz * pz
-  let h1 = ST.get () in
-  assert (fmont_as_nat h1 s1 == S.fmul (fmont_as_nat h0 qz) (fmont_as_nat h0 qz));
-  assert (fmont_as_nat h1 s2 == S.fmul (fmont_as_nat h0 pz) (fmont_as_nat h0 pz));
-
-  fmul u1 px s1;        // u1 = px * z2z2
-  fmul u2 qx s2;        // u2 = qx * z1z1
-  let h2 = ST.get () in
-  assert (fmont_as_nat h2 u1 == S.fmul (fmont_as_nat h0 px) (fmont_as_nat h1 s1));
-  assert (fmont_as_nat h2 u2 == S.fmul (fmont_as_nat h0 qx) (fmont_as_nat h1 s2));
-
-  fmul s1 qz s1;
-  fmul s1 py s1;
-  let h3 = ST.get () in
-  assert (fmont_as_nat h3 s1 ==
-    S.fmul (fmont_as_nat h0 py) (S.fmul (fmont_as_nat h0 qz) (fmont_as_nat h1 s1)));
-  Lib.NatMod.lemma_mul_mod_assoc #S.prime
-    (fmont_as_nat h0 py) (fmont_as_nat h0 qz) (fmont_as_nat h1 s1);
-
-  fmul s2 pz s2;
-  fmul s2 qy s2;
-  let h4 = ST.get () in
-  assert (fmont_as_nat h4 s2 ==
-    S.fmul (fmont_as_nat h0 qy) (S.fmul (fmont_as_nat h0 pz) (fmont_as_nat h1 s2)));
-  Lib.NatMod.lemma_mul_mod_assoc #S.prime
-    (fmont_as_nat h0 qy) (fmont_as_nat h0 pz) (fmont_as_nat h1 s2)
-
-
-inline_for_extraction noextract
-val point_add_hhh_uhh_h_r:
-    h:felem -> r:felem -> hhh:felem
-  -> u1:felem -> u2:felem -> s1:felem -> s2:felem ->
-  Stack unit
-  (requires fun h0 ->
-    live h0 h /\ live h0 r /\ live h0 hhh /\
-    live h0 u1 /\ live h0 u2 /\ live h0 s1 /\ live h0 s2 /\
+    live h t0 /\ live h t1 /\ live h t2 /\
+    live h t3 /\ live h t4 /\ live h p /\ live h q /\
     LowStar.Monotonic.Buffer.all_disjoint
-      [loc u1; loc u2; loc s1; loc s2; loc h; loc r; loc hhh] /\
-    as_nat h0 u1 < S.prime /\ as_nat h0 u2 < S.prime /\
-    as_nat h0 s1 < S.prime /\ as_nat h0 s2 < S.prime)
-  (ensures fun h0 _ h1 ->
-    modifies (loc h |+| loc r |+| loc u1 |+| loc hhh) h0 h1 /\
-    as_nat h1 h < S.prime /\ as_nat h1 r < S.prime /\
-    as_nat h1 u1 < S.prime /\ as_nat h1 hhh < S.prime /\
-    fmont_as_nat h1 h == S.fsub (fmont_as_nat h0 u2) (fmont_as_nat h0 u1) /\
-    fmont_as_nat h1 r == S.fsub (fmont_as_nat h0 s2) (fmont_as_nat h0 s1) /\
-    fmont_as_nat h1 u1 ==
-      S.fmul (fmont_as_nat h0 u1) (S.fmul (fmont_as_nat h1 h) (fmont_as_nat h1 h)) /\
-    fmont_as_nat h1 hhh ==
-      S.fmul (S.fmul (fmont_as_nat h1 h) (fmont_as_nat h1 h)) (fmont_as_nat h1 h))
-
-let point_add_hhh_uhh_h_r h r hhh u1 u2 s1 s2 =
-  let h0 = ST.get () in
-  fsub h u2 u1;     // h = u2 - u1
-  fsub r s2 s1;     // r = s2 - s1
-  let h1 = ST.get () in
-  assert (fmont_as_nat h1 h == S.fsub (fmont_as_nat h0 u2) (fmont_as_nat h0 u1));
-  assert (fmont_as_nat h1 r == S.fsub (fmont_as_nat h0 s2) (fmont_as_nat h0 s1));
-
-  fsqr hhh h;      // hh = h * h
-  fmul u1 hhh u1;  // u1hh = u1 * hh
-  fmul hhh h hhh   // hhh = hh * h
-
-
-inline_for_extraction noextract
-val point_add_x3: x3:felem -> hhh:felem -> u1:felem -> r:felem -> tmp:felem ->
-  Stack unit
-  (requires fun h0 ->
-    live h0 x3 /\ live h0 hhh /\ live h0 u1 /\ live h0 r /\ live h0 tmp /\
-    LowStar.Monotonic.Buffer.all_disjoint [loc x3; loc hhh; loc u1; loc r; loc tmp] /\
-    as_nat h0 hhh < S.prime /\ as_nat h0 u1 < S.prime /\ as_nat h0 r < S.prime)
-  (ensures fun h0 _ h1 -> modifies (loc x3 |+| loc tmp) h0 h1 /\
-    as_nat h1 x3 < S.prime /\
-    fmont_as_nat h1 x3 ==
-      S.fsub
-        (S.fsub (S.fmul (fmont_as_nat h0 r) (fmont_as_nat h0 r)) (fmont_as_nat h0 hhh))
-        (S.fmul 2 (fmont_as_nat h0 u1)))
-
-let point_add_x3 x3 hhh u1 r tmp =
-  fsqr x3 r;       // rr = r * r
-  fsub x3 x3 hhh;  // rr - hhh
-  fdouble tmp u1;  // 2 * u1
-  fsub x3 x3 tmp   // rr - hhh - 2 * u1
-
-
-inline_for_extraction noextract
-val point_add_y3: y3:felem -> s1:felem -> hhh:felem -> u1:felem -> x3:felem -> r:felem ->
-  Stack unit
-  (requires fun h ->
-    live h y3 /\ live h s1 /\ live h hhh /\ live h u1 /\ live h x3 /\ live h r /\
-    LowStar.Monotonic.Buffer.all_disjoint [loc y3; loc s1; loc hhh; loc u1; loc x3; loc r] /\
-    as_nat h s1 < S.prime /\ as_nat h hhh < S.prime /\
-    as_nat h u1 < S.prime /\ as_nat h x3 < S.prime /\ as_nat h r < S.prime)
-  (ensures fun h0 _ h1 -> modifies (loc y3 |+| loc u1) h0 h1 /\
-    as_nat h1 y3 < S.prime /\
-    fmont_as_nat h1 y3 =
-      S.fsub
-        (S.fmul (fmont_as_nat h0 r) (S.fsub (fmont_as_nat h0 u1) (fmont_as_nat h0 x3)))
-        (S.fmul (fmont_as_nat h0 s1) (fmont_as_nat h0 hhh)))
-
-let point_add_y3 y3 s1 hhh u1 x3 r =
-  fmul y3 s1 hhh;  // s1 * hhh
-  fsub u1 u1 x3;   // u1 - x3
-  fmul u1 r u1;    // r * (u1 - x3)
-  fsub y3 u1 y3    // r * (u1 - x3) - s1 * hhh
-
-
-inline_for_extraction noextract
-val point_add_z3: z3:felem -> z1:felem -> z2:felem -> h:felem -> Stack unit
-  (requires fun h0 ->
-    live h0 z3 /\ live h0 z1 /\ live h0 z2 /\ live h0 h /\
-    eq_or_disjoint z1 z3 /\ eq_or_disjoint z2 z3 /\ eq_or_disjoint z1 z2 /\
-    disjoint h z1 /\ disjoint h z2 /\ disjoint h z3 /\
-    as_nat h0 z1 < S.prime /\ as_nat h0 z2 < S.prime /\ as_nat h0 h < S.prime)
-  (ensures fun h0 _ h1 -> modifies (loc z3 |+| loc h) h0 h1 /\
-    as_nat h1 z3 < S.prime /\
-    fmont_as_nat h1 z3 ==
-      S.fmul (S.fmul (fmont_as_nat h0 h) (fmont_as_nat h0 z1)) (fmont_as_nat h0 z2))
-
-let point_add_z3 z3 z1 z2 h =
-  fmul h z1 h;
-  fmul z3 h z2
-
-
-inline_for_extraction noextract
-val point_add_no_point_at_inf:
-  p:point -> q:point -> res:point -> tmp:lbuffer uint64 32ul -> Stack unit
-  (requires fun h ->
-    live h p /\ live h q /\ live h res /\ live h tmp /\
-    eq_or_disjoint q res /\ disjoint p q /\ disjoint p tmp /\
-    disjoint q tmp /\ disjoint p res /\ disjoint res tmp /\
+      [loc t0; loc t1; loc t2; loc t3; loc t4 ] /\
+    eq_or_disjoint p q /\ disjoint p t0 /\ disjoint p t1 /\
+    disjoint p t2 /\ disjoint p t3 /\ disjoint p t4 /\
+    disjoint q t0 /\ disjoint q t1 /\ disjoint q t2 /\
+    disjoint q t3 /\ disjoint q t4 /\
     point_inv h p /\ point_inv h q)
-  (ensures fun h0 _ h1 -> modifies (loc tmp |+| loc res) h0 h1 /\
-    point_inv h1 res /\
-    from_mont_point (as_point_nat h1 res) == S.point_add_no_point_at_inf
-      (from_mont_point (as_point_nat h0 p)) (from_mont_point (as_point_nat h0 q)))
+  (ensures fun h0 _ h1 -> modifies (loc t0 |+| loc t1 |+| loc t2 |+| loc t3 |+| loc t4) h0 h1 /\
+    as_nat h1 t0 < S.prime /\ as_nat h1 t1 < S.prime /\
+    as_nat h1 t2 < S.prime /\ as_nat h1 t3 < S.prime /\
+    as_nat h1 t4 < S.prime /\
+    (let x1, y1, z1 = from_mont_point (as_point_nat h0 p) in
+    let x2, y2, z2 = from_mont_point (as_point_nat h0 q) in
+    let t0_s = S.fmul x1 x2 in
+    let t1_s = S.fmul y1 y2 in
+    let t2_s = S.fmul z1 z2 in
+    let t3_s = S.fadd x1 y1 in
+    let t4_s = S.fadd x2 y2 in
+    let t3_s = S.fmul t3_s t4_s in
+    let t4_s = S.fadd t0_s t1_s in
 
-let point_add_no_point_at_inf p q res tmp =
-  let z1 = getz p in
-  let z2 = getz q in
+    fmont_as_nat h1 t0 == t0_s /\ fmont_as_nat h1 t1 == t1_s /\
+    fmont_as_nat h1 t2 == t2_s /\ fmont_as_nat h1 t3 == t3_s /\
+    fmont_as_nat h1 t4 == t4_s))
 
-  let u1 = sub tmp 0ul 4ul in
-  let u2 = sub tmp 4ul 4ul in
-  let s1 = sub tmp 8ul 4ul in
-  let s2 = sub tmp 12ul 4ul in
-
-  let h = sub tmp 16ul 4ul in
-  let r = sub tmp 20ul 4ul in
-  let hhh = sub tmp 24ul 4ul in
-  let ftmp = sub tmp 28ul 4ul in
-
-  let x3 = getx res in
-  let y3 = gety res in
-  let z3 = getz res in
-
-  point_add_u12_s12 u1 u2 s1 s2 p q;
-  point_add_hhh_uhh_h_r h r hhh u1 u2 s1 s2;
-  point_add_x3 x3 hhh u1 r ftmp;
-  point_add_y3 y3 s1 hhh u1 x3 r;
-  point_add_z3 z3 z1 z2 h
+let point_add_1 t0 t1 t2 t3 t4 p q =
+  let x1, y1, z1 = getx p, gety p, getz p in
+  let x2, y2, z2 = getx q, gety q, getz q in
+  fmul t0 x1 x2;
+  fmul t1 y1 y2;
+  fmul t2 z1 z2;
+  fadd t3 x1 y1;
+  fadd t4 x2 y2;
+  fmul t3 t3 t4;
+  fadd t4 t0 t1
 
 
 inline_for_extraction noextract
-val point_add_condional_branch: p:point -> q:point -> res:point -> Stack unit
+val point_add_2 (t1 t2 t3 t4 t5:felem) (p q:point) : Stack unit
   (requires fun h ->
-    live h p /\ live h q /\ live h res /\
-    disjoint p res /\ disjoint q res /\ disjoint p q /\
-    point_inv h p /\ point_inv h q /\ point_inv h res)
-  (ensures  fun h0 _ h1 -> modifies (loc res) h0 h1 /\
-    point_inv h1 res /\
-   (let p = from_mont_point (as_point_nat h0 p) in
-    let q = from_mont_point (as_point_nat h0 q) in
-    let r = from_mont_point (as_point_nat h0 res) in
-    from_mont_point (as_point_nat h1 res) ==
-      (if S.is_point_at_inf q then p else if S.is_point_at_inf p then q else r)))
+    live h t1 /\ live h t2 /\ live h t3 /\ live h t4 /\ live h t5 /\
+    live h p /\ live h q /\
+    LowStar.Monotonic.Buffer.all_disjoint [ loc t1; loc t2; loc t3; loc t4; loc t5 ] /\
+    eq_or_disjoint p q /\ disjoint p t1 /\ disjoint p t2 /\
+    disjoint p t3 /\ disjoint p t4 /\ disjoint p t5 /\
+    disjoint q t1 /\ disjoint q t2 /\ disjoint q t3 /\
+    disjoint q t4 /\ disjoint q t5 /\
+    point_inv h p /\ point_inv h q /\
+    as_nat h t1 < S.prime /\ as_nat h t2 < S.prime /\
+    as_nat h t3 < S.prime /\ as_nat h t4 < S.prime)
+  (ensures  fun h0 _ h1 -> modifies (loc t3 |+| loc t4 |+| loc t5) h0 h1 /\
+    as_nat h1 t3 < S.prime /\ as_nat h1 t4 < S.prime /\ as_nat h1 t5 < S.prime /\
+    (let x1, y1, z1 = from_mont_point (as_point_nat h0 p) in
+    let x2, y2, z2 = from_mont_point (as_point_nat h0 q) in
+    let t1_s = fmont_as_nat h0 t1 in
+    let t2_s = fmont_as_nat h0 t2 in
+    let t3_s = fmont_as_nat h0 t3 in
+    let t4_s = fmont_as_nat h0 t4 in
+    let t3_s = S.fsub t3_s t4_s in
+    let t4_s = S.fadd y1 z1 in
+    let t5_s = S.fadd y2 z2 in
+    let t4_s = S.fmul t4_s t5_s in
+    let t5_s = S.fadd t1_s t2_s in
+    let t4_s = S.fsub t4_s t5_s in
 
-let point_add_condional_branch p q res =
-  copy_point_conditional res q p;
-  copy_point_conditional res p q
+    fmont_as_nat h1 t3 == t3_s /\ fmont_as_nat h1 t4 == t4_s /\
+    fmont_as_nat h1 t5 == t5_s))
+
+let point_add_2 t1 t2 t3 t4 t5 p q =
+  let y1, z1 = gety p, getz p in
+  let y2, z2 = gety q, getz q in
+  fsub t3 t3 t4;
+  fadd t4 y1 z1;
+  fadd t5 y2 z2;
+  fmul t4 t4 t5;
+  fadd t5 t1 t2;
+  fsub t4 t4 t5
+
+
+inline_for_extraction noextract
+val point_add_3 (x3 y3 t0 t2:felem) (p q:point) : Stack unit
+  (requires fun h ->
+    live h x3 /\ live h y3 /\ live h t0 /\ live h t2 /\
+    live h p /\ live h q /\
+    LowStar.Monotonic.Buffer.all_disjoint [ loc x3; loc y3; loc t0; loc t2 ] /\
+    eq_or_disjoint p q /\ disjoint p x3 /\ disjoint p y3 /\
+    disjoint p t0 /\ disjoint p t2 /\ disjoint q x3 /\
+    disjoint q y3 /\ disjoint q t0 /\ disjoint q t2 /\
+    point_inv h p /\ point_inv h q /\
+    as_nat h t0 < S.prime /\ as_nat h t2 < S.prime)
+  (ensures  fun h0 _ h1 -> modifies (loc x3 |+| loc y3) h0 h1 /\
+    as_nat h1 x3 < S.prime /\ as_nat h1 y3 < S.prime /\
+    (let x1, y1, z1 = from_mont_point (as_point_nat h0 p) in
+    let x2, y2, z2 = from_mont_point (as_point_nat h0 q) in
+    let t0_s = fmont_as_nat h0 t0 in
+    let t2_s = fmont_as_nat h0 t2 in
+    let x3_s = S.fadd x1 z1 in
+    let y3_s = S.fadd x2 z2 in
+    let x3_s = S.fmul x3_s y3_s in
+    let y3_s = S.fadd t0_s t2_s in
+    let y3_s = S.fsub x3_s y3_s in
+    fmont_as_nat h1 x3 == x3_s /\ fmont_as_nat h1 y3 == y3_s))
+
+let point_add_3 x3 y3 t0 t2 p q =
+  let x1, z1 = getx p, getz p in
+  let x2, z2 = getx q, getz q in
+  fadd x3 x1 z1;
+  fadd y3 x2 z2;
+  fmul x3 x3 y3;
+  fadd y3 t0 t2;
+  fsub y3 x3 y3
+
+
+inline_for_extraction noextract
+val point_add_4 (x3 y3 z3 t1 t2:felem) : Stack unit
+  (requires fun h ->
+    live h x3 /\ live h y3 /\ live h z3 /\ live h t1 /\ live h t2 /\
+    LowStar.Monotonic.Buffer.all_disjoint [ loc x3; loc y3; loc z3; loc t1; loc t2 ] /\
+    as_nat h t1 < S.prime /\ as_nat h t2 < S.prime /\ as_nat h y3 < S.prime)
+  (ensures  fun h0 _ h1 -> modifies (loc x3 |+| loc y3 |+| loc z3) h0 h1 /\
+    as_nat h1 x3 < S.prime /\ as_nat h1 y3 < S.prime /\ as_nat h1 z3 < S.prime /\
+    (let t1_s = fmont_as_nat h0 t1 in
+    let t2_s = fmont_as_nat h0 t2 in
+    let y3_s = fmont_as_nat h0 y3 in
+    let z3_s = S.fmul S.b_coeff t2_s in
+    let x3_s = S.fsub y3_s z3_s in
+    let z3_s = S.fadd x3_s x3_s in
+    let x3_s = S.fadd x3_s z3_s in
+    let z3_s = S.fsub t1_s x3_s in
+    let x3_s = S.fadd t1_s x3_s in
+    let y3_s = S.fmul S.b_coeff y3_s in
+    fmont_as_nat h1 x3 == x3_s /\ fmont_as_nat h1 y3 == y3_s /\ fmont_as_nat h1 z3 == z3_s))
+
+let point_add_4 x3 y3 z3 t1 t2 =
+  fmul_by_b_coeff z3 t2;
+  fsub x3 y3 z3;
+  fdouble z3 x3;
+  fadd x3 x3 z3;
+  fsub z3 t1 x3;
+  fadd x3 t1 x3;
+  fmul_by_b_coeff y3 y3
+
+
+inline_for_extraction noextract
+val point_add_5 (x3 y3 z3 t0 t1 t2:felem) : Stack unit
+  (requires fun h ->
+    live h x3 /\ live h y3 /\ live h z3 /\
+    live h t0 /\ live h t1 /\ live h t2 /\
+    LowStar.Monotonic.Buffer.all_disjoint [ loc x3; loc y3; loc z3; loc t0; loc t1; loc t2 ] /\
+    as_nat h y3 < S.prime /\ as_nat h t0 < S.prime /\
+    as_nat h t1 < S.prime /\ as_nat h t2 < S.prime)
+  (ensures  fun h0 _ h1 -> modifies (loc y3 |+| loc t1 |+| loc t2) h0 h1 /\
+    as_nat h1 t1 < S.prime /\ as_nat h1 t2 < S.prime /\ as_nat h1 y3 < S.prime /\
+    (let t0_s = fmont_as_nat h0 t0 in
+    let t1_s = fmont_as_nat h0 t1 in
+    let t2_s = fmont_as_nat h0 t2 in
+    let y3_s = fmont_as_nat h0 y3 in
+    let t1_s = S.fadd t2_s t2_s in
+    let t2_s = S.fadd t1_s t2_s in
+    let y3_s = S.fsub y3_s t2_s in
+    let y3_s = S.fsub y3_s t0_s in
+    let t1_s = S.fadd y3_s y3_s in
+    fmont_as_nat h1 t1 == t1_s /\ fmont_as_nat h1 t2 == t2_s /\ fmont_as_nat h1 y3 == y3_s))
+
+let point_add_5 x3 y3 z3 t0 t1 t2 =
+  fdouble t1 t2;
+  fadd t2 t1 t2;
+  fsub y3 y3 t2;
+  fsub y3 y3 t0;
+  fdouble t1 y3
+
+
+inline_for_extraction noextract
+val point_add_6 (x3 y3 z3 t0 t1 t2 t4:felem) : Stack unit
+  (requires fun h ->
+    live h x3 /\ live h y3 /\ live h z3 /\
+    live h t0 /\ live h t1 /\ live h t2 /\ live h t4 /\
+    LowStar.Monotonic.Buffer.all_disjoint
+      [ loc x3; loc y3; loc z3; loc t0; loc t1; loc t2; loc t4 ] /\
+    as_nat h y3 < S.prime /\ as_nat h t0 < S.prime /\
+    as_nat h t1 < S.prime /\ as_nat h t2 < S.prime /\
+    as_nat h t4 < S.prime)
+  (ensures  fun h0 _ h1 -> modifies (loc y3 |+| loc t0 |+| loc t1 |+| loc t2) h0 h1 /\
+    as_nat h1 t0 < S.prime /\ as_nat h1 t1 < S.prime /\
+    as_nat h1 t2 < S.prime /\ as_nat h1 y3 < S.prime /\
+    (let t0_s = fmont_as_nat h0 t0 in
+    let t1_s = fmont_as_nat h0 t1 in
+    let t2_s = fmont_as_nat h0 t2 in
+    let t4_s = fmont_as_nat h0 t4 in
+    let y3_s = fmont_as_nat h0 y3 in
+    let y3_s = S.fadd t1_s y3_s in
+    let t1_s = S.fadd t0_s t0_s in
+    let t0_s = S.fadd t1_s t0_s in
+    let t0_s = S.fsub t0_s t2_s in
+    let t1_s = S.fmul t4_s y3_s in
+    let t2_s = S.fmul t0_s y3_s in
+    fmont_as_nat h1 t0 == t0_s /\ fmont_as_nat h1 t1 == t1_s /\
+    fmont_as_nat h1 t2 == t2_s /\ fmont_as_nat h1 y3 == y3_s))
+
+let point_add_6 x3 y3 z3 t0 t1 t2 t4 =
+  fadd y3 t1 y3;
+  fdouble t1 t0;
+  fadd t0 t1 t0;
+  fsub t0 t0 t2;
+  fmul t1 t4 y3;
+  fmul t2 t0 y3
+
+
+inline_for_extraction noextract
+val point_add_7 (x3 y3 z3 t0 t1 t2 t3 t4:felem) : Stack unit
+  (requires fun h ->
+    live h x3 /\ live h y3 /\ live h z3 /\
+    live h t0 /\ live h t1 /\ live h t2 /\ live h t3 /\ live h t4 /\
+    LowStar.Monotonic.Buffer.all_disjoint
+      [ loc x3; loc y3; loc z3; loc t0; loc t1; loc t2; loc t3; loc t4 ] /\
+    as_nat h x3 < S.prime /\ as_nat h z3 < S.prime /\
+    as_nat h t0 < S.prime /\ as_nat h t1 < S.prime /\
+    as_nat h t2 < S.prime /\ as_nat h t3 < S.prime /\ as_nat h t4 < S.prime)
+  (ensures  fun h0 _ h1 -> modifies (loc x3 |+| loc y3 |+| loc z3 |+| loc t1) h0 h1 /\
+    as_nat h1 x3 < S.prime /\ as_nat h1 y3 < S.prime /\
+    as_nat h1 z3 < S.prime /\ as_nat h1 t1 < S.prime /\
+    (let x3_s = fmont_as_nat h0 x3 in
+    let z3_s = fmont_as_nat h0 z3 in
+    let t0_s = fmont_as_nat h0 t0 in
+    let t1_s = fmont_as_nat h0 t1 in
+    let t2_s = fmont_as_nat h0 t2 in
+    let t3_s = fmont_as_nat h0 t3 in
+    let t4_s = fmont_as_nat h0 t4 in
+    let y3_s = S.fmul x3_s z3_s in
+    let y3_s = S.fadd y3_s t2_s in
+    let x3_s = S.fmul t3_s x3_s in
+    let x3_s = S.fsub x3_s t1_s in
+    let z3_s = S.fmul t4_s z3_s in
+    let t1_s = S.fmul t3_s t0_s in
+    let z3_s = S.fadd z3_s t1_s in
+    fmont_as_nat h1 x3 == x3_s /\ fmont_as_nat h1 y3 == y3_s /\
+    fmont_as_nat h1 z3 == z3_s /\ fmont_as_nat h1 t1 == t1_s))
+
+let point_add_7 x3 y3 z3 t0 t1 t2 t3 t4 =
+  fmul y3 x3 z3;
+  fadd y3 y3 t2;
+  fmul x3 t3 x3;
+  fsub x3 x3 t1;
+  fmul z3 t4 z3;
+  fmul t1 t3 t0;
+  fadd z3 z3 t1
 
 
 [@CInline]
 let point_add p q res tmp =
-  point_add_no_point_at_inf p q res tmp;
-  point_add_condional_branch p q res
+  let x3, y3, z3 = getx res, gety res, getz res in
+  let t0 = sub tmp 0ul 4ul in
+  let t1 = sub tmp 4ul 4ul in
+  let t2 = sub tmp 8ul 4ul in
+  let t3 = sub tmp 12ul 4ul in
+  let t4 = sub tmp 16ul 4ul in
+  let t5 = sub tmp 20ul 4ul in
+  point_add_1 t0 t1 t2 t3 t4 p q;
+  point_add_2 t1 t2 t3 t4 t5 p q;
+  point_add_3 x3 y3 t0 t2 p q;
+  point_add_4 x3 y3 z3 t1 t2;
+  point_add_5 x3 y3 z3 t0 t1 t2;
+  point_add_6 x3 y3 z3 t0 t1 t2 t4;
+  point_add_7 x3 y3 z3 t0 t1 t2 t3 t4
