code/ecdsap256/Hacl.Impl.P256.PointDouble.fst
@@ -17,160 +17,194 @@ module SM = Hacl.Spec.P256.Montgomery
 #set-options "--z3rlimit 50 --ifuel 0 --fuel 0"
 
 inline_for_extraction noextract
-val point_double_a_b_g_d:
-    p:point
-  -> alpha:felem -> beta:felem -> gamma:felem -> delta:felem
-  -> tmp:felem ->
-  Stack unit
+val point_double_1 (t0 t1 t2 t3 t4:felem) (p:point) : Stack unit
   (requires fun h ->
-    live h p /\ live h alpha /\ live h beta /\
-    live h gamma /\ live h delta /\ live h tmp /\
+    live h t0 /\ live h t1 /\ live h t2 /\
+    live h t3 /\ live h t4 /\ live h p /\
     LowStar.Monotonic.Buffer.all_disjoint
-      [loc p; loc alpha; loc beta; loc gamma; loc delta; loc tmp] /\
+      [loc t0; loc t1; loc t2; loc t3; loc t4; loc p ] /\
     point_inv h p)
-  (ensures fun h0 _ h1 ->
-    modifies (loc alpha |+| loc beta |+| loc gamma |+| loc delta |+| loc tmp) h0 h1 /\
-    as_nat h1 alpha < S.prime /\ as_nat h1 beta < S.prime /\
-    as_nat h1 gamma < S.prime /\ as_nat h1 delta < S.prime /\
-   (let x, y, z = from_mont_point (as_point_nat h0 p) in
-    fmont_as_nat h1 delta = S.fmul z z /\
-    fmont_as_nat h1 gamma = S.fmul y y /\
-    fmont_as_nat h1 beta = S.fmul x (fmont_as_nat h1 gamma) /\
-    fmont_as_nat h1 alpha =
-      S.fmul (S.fmul 3 (S.fsub x (fmont_as_nat h1 delta))) (S.fadd x (fmont_as_nat h1 delta))))
+  (ensures fun h0 _ h1 -> modifies (loc t0 |+| loc t1 |+| loc t2 |+| loc t3 |+| loc t4) h0 h1 /\
+    as_nat h1 t0 < S.prime /\ as_nat h1 t1 < S.prime /\
+    as_nat h1 t2 < S.prime /\ as_nat h1 t3 < S.prime /\
+    as_nat h1 t4 < S.prime /\
+    (let x, y, z = from_mont_point (as_point_nat h0 p) in
+    let t0_s = S.fmul x x in
+    let t1_s = S.fmul y y in
+    let t2_s = S.fmul z z in
+    let t3_s = S.fmul x y in
+    let t3_s = S.fadd t3_s t3_s in
+    let t4_s = S.fmul y z in
+    fmont_as_nat h1 t0 == t0_s /\ fmont_as_nat h1 t1 == t1_s /\
+    fmont_as_nat h1 t2 == t2_s /\ fmont_as_nat h1 t3 == t3_s /\
+    fmont_as_nat h1 t4 == t4_s))
 
-let point_double_a_b_g_d p alpha beta gamma delta tmp =
-  let px = getx p in
-  let py = gety p in
-  let pz = getz p in
-
-  let h0 = ST.get () in
-  fsqr delta pz;      // delta = z * z
-  fsqr gamma py;      // gamma = y * y
-  fmul beta px gamma; // beta = x * gamma
-  let h1 = ST.get () in
-  assert (fmont_as_nat h1 delta = S.fmul (fmont_as_nat h0 pz) (fmont_as_nat h0 pz));
-  assert (fmont_as_nat h1 gamma = S.fmul (fmont_as_nat h0 py) (fmont_as_nat h0 py));
-  assert (fmont_as_nat h1 beta = S.fmul (fmont_as_nat h0 px) (fmont_as_nat h1 gamma));
-
-  fsub alpha px delta;   // a0 = x - delta
-  let h2 = ST.get () in
-  assert (fmont_as_nat h2 alpha = S.fsub (fmont_as_nat h0 px) (fmont_as_nat h1 delta));
-  fmul_by_3 tmp alpha;
-  let h3 = ST.get () in
-  assert (fmont_as_nat h3 tmp = S.fmul 3 (fmont_as_nat h2 alpha));
-  fadd alpha px delta;   // a1 = x + delta
-  let h4 = ST.get () in
-  assert (fmont_as_nat h4 alpha = S.fadd (fmont_as_nat h0 px) (fmont_as_nat h1 delta));
-  fmul alpha tmp alpha
+let point_double_1 t0 t1 t2 t3 t4 p =
+  let x, y, z = getx p, gety p, getz p in
+  fsqr t0 x;
+  fsqr t1 y;
+  fsqr t2 z;
+  fmul t3 x y;
+  fdouble t3 t3;
+  fmul t4 y z
 
 
 inline_for_extraction noextract
-val point_double_x3: x3:felem -> alpha:felem -> beta:felem -> tmp:felem ->
-  Stack unit
+val point_double_2 (x3 y3 z3 t2:felem) : Stack unit
   (requires fun h ->
-    live h x3 /\ live h alpha /\ live h beta /\ live h tmp /\
-    LowStar.Monotonic.Buffer.all_disjoint
-      [loc x3; loc alpha; loc beta; loc tmp] /\
-    as_nat h alpha < S.prime /\ as_nat h beta < S.prime)
-  (ensures fun h0 _ h1 -> modifies (loc x3 |+| loc beta |+| loc tmp) h0 h1 /\
-    as_nat h1 beta < S.prime /\ as_nat h1 x3 < S.prime /\
-    fmont_as_nat h1 beta == S.fmul 4 (fmont_as_nat h0 beta) /\
-    fmont_as_nat h1 x3 == S.fsub (S.fmul (fmont_as_nat h0 alpha) (fmont_as_nat h0 alpha))
-      (S.fmul 8 (fmont_as_nat h0 beta)))
+    live h x3 /\ live h y3 /\ live h z3 /\ live h t2 /\
+    LowStar.Monotonic.Buffer.all_disjoint [ loc x3; loc y3; loc z3; loc t2 ] /\
+    as_nat h z3 < S.prime /\ as_nat h t2 < S.prime)
+  (ensures  fun h0 _ h1 -> modifies (loc x3 |+| loc y3 |+| loc z3) h0 h1 /\
+    as_nat h1 x3 < S.prime /\ as_nat h1 y3 < S.prime /\ as_nat h1 z3 < S.prime /\
+    (let z3_s = fmont_as_nat h0 z3 in
+    let t2_s = fmont_as_nat h0 t2 in
+    let z3_s = S.fadd z3_s z3_s in
+    let y3_s = S.fmul S.b_coeff t2_s in
+    let y3_s = S.fsub y3_s z3_s in
+    let x3_s = S.fadd y3_s y3_s in
+    let y3_s = S.fadd x3_s y3_s in
+    fmont_as_nat h1 x3 == x3_s /\ fmont_as_nat h1 y3 == y3_s /\
+    fmont_as_nat h1 z3 == z3_s))
 
-let point_double_x3 x3 alpha beta tmp =
-  let h0 = ST.get () in
-  fsqr x3 alpha;          // x3 = alpha * alpha
-  fmul_by_4 beta beta;    // beta = 4 * beta
-  let h1 = ST.get () in
-  assert (fmont_as_nat h1 x3 = S.fmul (fmont_as_nat h0 alpha) (fmont_as_nat h0 alpha));
-  assert (fmont_as_nat h1 beta = S.fmul 4 (fmont_as_nat h0 beta));
-  fdouble tmp beta;      // tmp = 8 * beta
-  let h2 = ST.get () in
-  assert (fmont_as_nat h2 tmp = S.fmul 2 (S.fmul 4 (fmont_as_nat h0 beta)));
-  Math.Lemmas.lemma_mod_mul_distr_r 2 (4 * fmont_as_nat h0 beta) S.prime;
-  assert (fmont_as_nat h2 tmp = S.fmul 8 (fmont_as_nat h0 beta));
-  fsub x3 x3 tmp         // x3 = alpha * alpha - 8 * beta
+let point_double_2 x3 y3 z3 t2 =
+  fdouble z3 z3;
+  fmul_by_b_coeff y3 t2;
+  fsub y3 y3 z3;
+  fdouble x3 y3;
+  fadd y3 x3 y3
 
 
 inline_for_extraction noextract
-val point_double_z3: z3:felem -> py:felem -> pz:felem -> gamma:felem -> delta:felem ->
-  Stack unit
+val point_double_3 (x3 y3 t1 t2 t3:felem) : Stack unit
   (requires fun h ->
-    live h z3 /\ live h py /\ live h pz /\ live h gamma /\ live h delta /\
-    eq_or_disjoint pz z3 /\ disjoint z3 gamma /\ disjoint z3 delta /\
-    disjoint py z3 /\ disjoint py pz /\
-    as_nat h gamma < S.prime /\ as_nat h delta < S.prime /\
-    as_nat h py < S.prime /\ as_nat h pz < S.prime)
-  (ensures fun h0 _ h1 -> modifies (loc z3) h0 h1 /\
-    as_nat h1 z3 < S.prime /\
-   (let yz = S.fadd (fmont_as_nat h0 py) (fmont_as_nat h0 pz) in
-    fmont_as_nat h1 z3 =
-      S.fsub (S.fsub (S.fmul yz yz) (fmont_as_nat h0 delta)) (fmont_as_nat h0 gamma)))
+    live h x3 /\ live h y3 /\ live h t1 /\ live h t2 /\ live h t3 /\
+    LowStar.Monotonic.Buffer.all_disjoint [ loc x3; loc y3; loc t1; loc t2; loc t3 ] /\
+    as_nat h t1 < S.prime /\ as_nat h t2 < S.prime /\
+    as_nat h t3 < S.prime /\ as_nat h y3 < S.prime)
+  (ensures  fun h0 _ h1 -> modifies (loc x3 |+| loc y3 |+| loc t2 |+| loc t3) h0 h1 /\
+    as_nat h1 x3 < S.prime /\ as_nat h1 y3 < S.prime /\
+    as_nat h1 t2 < S.prime /\ as_nat h1 t3 < S.prime /\
+    (let t1_s = fmont_as_nat h0 t1 in
+    let t2_s = fmont_as_nat h0 t2 in
+    let t3_s = fmont_as_nat h0 t3 in
+    let y3_s = fmont_as_nat h0 y3 in
+    let x3_s = S.fsub t1_s y3_s in
+    let y3_s = S.fadd t1_s y3_s in
+    let y3_s = S.fmul x3_s y3_s in
+    let x3_s = S.fmul x3_s t3_s in
+    let t3_s = S.fadd t2_s t2_s in
+    let t2_s = S.fadd t2_s t3_s in
 
-let point_double_z3 z3 py pz gamma delta =
-  let h0 = ST.get () in
-  fadd z3 py pz;  // z3 = py + pz
-  fsqr z3 z3;     // z3 = (py + pz) * (py + pz)
-  let h1 = ST.get () in
-  assert (let yz = S.fadd (fmont_as_nat h0 py) (fmont_as_nat h0 pz) in
-    fmont_as_nat h1 z3 = S.fmul yz yz);
+    fmont_as_nat h1 x3 == x3_s /\ fmont_as_nat h1 y3 == y3_s /\
+    fmont_as_nat h1 t2 == t2_s /\ fmont_as_nat h1 t3 == t3_s))
 
-  fsub z3 z3 delta;  // z3 = (py + pz) ** 2 - delta
-  fsub z3 z3 gamma   // z3 = (py + pz) ** 2 - delta - gamma
+let point_double_3 x3 y3 t1 t2 t3 =
+  fsub x3 t1 y3;
+  fadd y3 t1 y3;
+  fmul y3 x3 y3;
+  fmul x3 x3 t3;
+  fdouble t3 t2;
+  fadd t2 t2 t3
 
 
 inline_for_extraction noextract
-val point_double_y3: y3:felem -> x3:felem -> alpha:felem -> gamma:felem -> beta:felem ->
-  Stack unit
+val point_double_4 (z3 t0 t2 t3:felem) : Stack unit
   (requires fun h ->
-    live h y3 /\ live h x3 /\ live h alpha /\ live h gamma /\ live h beta /\
-    LowStar.Monotonic.Buffer.all_disjoint
-      [loc y3; loc x3; loc alpha; loc gamma; loc beta] /\
-    as_nat h x3 < S.prime /\ as_nat h alpha < S.prime /\
-    as_nat h gamma < S.prime /\ as_nat h beta < S.prime)
-  (ensures fun h0 _ h1 -> modifies (loc y3 |+| loc gamma) h0 h1 /\
-    as_nat h1 y3 < S.prime /\
-    fmont_as_nat h1 y3 ==
-    S.fsub
-      (S.fmul (fmont_as_nat h0 alpha) (S.fsub (fmont_as_nat h0 beta) (fmont_as_nat h0 x3)))
-      (S.fmul (S.fmul 8 (fmont_as_nat h0 gamma)) (fmont_as_nat h0 gamma)))
+    live h z3 /\ live h t0 /\ live h t2 /\ live h t3 /\
+    LowStar.Monotonic.Buffer.all_disjoint [ loc z3; loc t0; loc t2; loc t3 ] /\
+    as_nat h z3 < S.prime /\ as_nat h t0 < S.prime /\ as_nat h t2 < S.prime)
+  (ensures  fun h0 _ h1 -> modifies (loc z3 |+| loc t3) h0 h1 /\
+    as_nat h1 z3 < S.prime /\ as_nat h1 t3 < S.prime /\
+    (let z3_s = fmont_as_nat h0 z3 in
+    let t0_s = fmont_as_nat h0 t0 in
+    let t2_s = fmont_as_nat h0 t2 in
+    let z3_s = S.fmul S.b_coeff z3_s in
+    let z3_s = S.fsub z3_s t2_s in
+    let z3_s = S.fsub z3_s t0_s in
+    let t3_s = S.fadd z3_s z3_s in
+    let z3_s = S.fadd z3_s t3_s in
+    fmont_as_nat h1 z3 == z3_s /\ fmont_as_nat h1 t3 == t3_s))
 
-let point_double_y3 y3 x3 alpha gamma beta =
-  let h0 = ST.get () in
-  fsub y3 beta x3;      // y3 = beta - x3
-  fmul y3 alpha y3;     // y3 = alpha * (beta - x3)
-  let h1 = ST.get () in
-  assert (fmont_as_nat h1 y3 =
-    S.fmul (fmont_as_nat h0 alpha) (S.fsub (fmont_as_nat h0 beta) (fmont_as_nat h0 x3)));
+let point_double_4 z3 t0 t2 t3 =
+  fmul_by_b_coeff z3 z3;
+  fsub z3 z3 t2;
+  fsub z3 z3 t0;
+  fdouble t3 z3;
+  fadd z3 z3 t3
 
-  fsqr gamma gamma;
-  fmul_by_8 gamma gamma; // gamma = 8 * gamma * gamma
-  let h2 = ST.get () in
-  assert (let g = fmont_as_nat h0 gamma in
-    fmont_as_nat h2 gamma == S.fmul 8 (S.fmul g g));
-  Lib.NatMod.lemma_mul_mod_assoc #S.prime 8 (fmont_as_nat h0 gamma) (fmont_as_nat h0 gamma);
-  fsub y3 y3 gamma       // y3 = alpha * (beta - x3) - 8 * gamma * gamma
+
+inline_for_extraction noextract
+val point_double_5 (y3 z3 t0 t2 t3:felem) : Stack unit
+  (requires fun h ->
+    live h y3 /\ live h z3 /\ live h t0 /\ live h t2 /\ live h t3 /\
+    LowStar.Monotonic.Buffer.all_disjoint [ loc y3; loc z3; loc t0; loc t2; loc t3 ] /\
+    as_nat h y3 < S.prime /\ as_nat h z3 < S.prime /\
+    as_nat h t0 < S.prime /\ as_nat h t2 < S.prime)
+  (ensures  fun h0 _ h1 -> modifies (loc y3 |+| loc t0 |+| loc t3) h0 h1 /\
+    as_nat h1 y3 < S.prime /\ as_nat h1 t3 < S.prime /\
+    (let t0_s = fmont_as_nat h0 t0 in
+    let t2_s = fmont_as_nat h0 t2 in
+    let y3_s = fmont_as_nat h0 y3 in
+    let z3_s = fmont_as_nat h0 z3 in
+    let t3_s = S.fadd t0_s t0_s in
+    let t0_s = S.fadd t3_s t0_s in
+    let t0_s = S.fsub t0_s t2_s in
+    let t0_s = S.fmul t0_s z3_s in
+    let y3_s = S.fadd y3_s t0_s in
+    fmont_as_nat h1 y3 == y3_s /\ fmont_as_nat h1 t0 == t0_s /\ fmont_as_nat h1 t3 == t3_s))
+
+let point_double_5 y3 z3 t0 t2 t3 =
+  fdouble t3 t0;
+  fadd t0 t3 t0;
+  fsub t0 t0 t2;
+  fmul t0 t0 z3;
+  fadd y3 y3 t0
+
+
+inline_for_extraction noextract
+val point_double_6 (x3 z3 t0 t1 t4:felem) : Stack unit
+  (requires fun h ->
+    live h x3 /\ live h z3 /\ live h t0 /\ live h t1 /\ live h t4 /\
+    LowStar.Monotonic.Buffer.all_disjoint [ loc x3; loc z3; loc t0; loc t1; loc t4 ] /\
+    as_nat h x3 < S.prime /\ as_nat h z3 < S.prime /\
+    as_nat h t1 < S.prime /\ as_nat h t4 < S.prime)
+  (ensures  fun h0 _ h1 -> modifies (loc x3 |+| loc z3 |+| loc t0) h0 h1 /\
+    as_nat h1 x3 < S.prime /\ as_nat h1 z3 < S.prime /\ as_nat h1 t0 < S.prime /\
+    (let t1_s = fmont_as_nat h0 t1 in
+    let t4_s = fmont_as_nat h0 t4 in
+    let x3_s = fmont_as_nat h0 x3 in
+    let z3_s = fmont_as_nat h0 z3 in
+    let t0_s = S.fadd t4_s t4_s in
+    let z3_s = S.fmul t0_s z3_s in
+    let x3_s = S.fsub x3_s z3_s in
+    let z3_s = S.fmul t0_s t1_s in
+    let z3_s = S.fadd z3_s z3_s in
+    let z3_s = S.fadd z3_s z3_s in
+    fmont_as_nat h1 z3 == z3_s /\ fmont_as_nat h1 x3 == x3_s /\ fmont_as_nat h1 t0 == t0_s))
+
+let point_double_6 x3 z3 t0 t1 t4 =
+  fdouble t0 t4;
+  fmul z3 t0 z3;
+  fsub x3 x3 z3;
+  fmul z3 t0 t1;
+  fdouble z3 z3;
+  fdouble z3 z3
 
 
 [@CInline]
 let point_double p res tmp =
-  let px = getx p in
-  let py = gety p in
-  let pz = getz p in
-
-  let x3 = getx res in
-  let y3 = gety res in
-  let z3 = getz res in
-
-  let delta = sub tmp 0ul 4ul in
-  let gamma = sub tmp 4ul 4ul in
-  let beta  = sub tmp 8ul 4ul in
-  let alpha = sub tmp 12ul 4ul in
-  let ftmp  = sub tmp 16ul 4ul in
-
-  point_double_a_b_g_d p alpha beta gamma delta ftmp;
-  point_double_x3 x3 alpha beta ftmp;
-  point_double_z3 z3 py pz gamma delta;
-  point_double_y3 y3 x3 alpha gamma beta
+  let x, z = getx p, getz p in
+  let x3, y3, z3 = getx res, gety res, getz res in
+  let t0 = sub tmp 0ul 4ul in
+  let t1 = sub tmp 4ul 4ul in
+  let t2 = sub tmp 8ul 4ul in
+  let t3 = sub tmp 12ul 4ul in
+  let t4 = sub tmp 16ul 4ul in
+  point_double_1 t0 t1 t2 t3 t4 p;
+  fmul z3 x z;
+  point_double_2 x3 y3 z3 t2;
+  point_double_3 x3 y3 t1 t2 t3;
+  point_double_4 z3 t0 t2 t3;
+  point_double_5 y3 z3 t0 t2 t3;
+  point_double_6 x3 z3 t0 t1 t4
