code/ecdsap256/Hacl.Impl.P256.Verify.fst
@@ -84,28 +84,27 @@ val ecdsa_verification_getx: x:felem -> pk:point -> u1:felem -> u2:felem -> Stac
     disjoint pk u1 /\ disjoint pk u2 /\
     point_inv h pk /\ as_nat h u1 < pow2 256 /\ as_nat h u2 < pow2 256)
   (ensures fun h0 b h1 -> modifies (loc x) h0 h1 /\
-    as_nat h1 x < S.prime /\
-   (let res = S.norm_jacob_point
-     (S.point_mul_double_g (as_nat h0 u1) (as_nat h0 u2) (as_point_nat h0 pk)) in
-    let (rx, _, _) = res in
-    b == not (S.is_point_at_inf res) /\ as_nat h1 x == rx % S.order))
+   (let res_proj = S.point_mul_double_g (as_nat h0 u1) (as_nat h0 u2) (as_point_nat h0 pk) in
+    let (rx, _) = S.to_aff_point res_proj in
+    b == not (S.is_point_at_inf res_proj) /\ as_nat h1 x == rx % S.order))
 
 let ecdsa_verification_getx x pk u1 u2 =
   push_frame ();
-  let res = create_point () in
+  let res_proj = create_point () in
   let h0 = ST.get () in
-  point_mul_double_g res u1 u2 pk;
+  point_mul_double_g res_proj u1 u2 pk;
   let h1 = ST.get () in
-  assert (from_mont_point (as_point_nat h1 res) ==
+  assert (from_mont_point (as_point_nat h1 res_proj) ==
     S.point_mul_double_g (as_nat h0 u1) (as_nat h0 u2) (as_point_nat h0 pk));
-  norm_jacob_point res res;
+  let is_res_point_at_inf = is_point_at_inf_vartime res_proj in
+  assert (is_res_point_at_inf == S.is_point_at_inf (from_mont_point (as_point_nat h1 res_proj)));
+  to_aff_point_x x res_proj;
   let h2 = ST.get () in
-  assert (as_point_nat h2 res ==
-    S.norm_jacob_point (from_mont_point (as_point_nat h1 res)));
-  let is_res_point_at_inf = is_point_at_inf_vartime res in
-  assert (is_res_point_at_inf == S.is_point_at_inf (as_point_nat h2 res));
-  let res_x = getx res in
-  qmod_short x res_x;
+  qmod_short x x;
+  let h3 = ST.get () in
+  assert (as_nat h2 x == fst (S.to_aff_point
+    (S.point_mul_double_g (as_nat h0 u1) (as_nat h0 u2) (as_point_nat h0 pk))));
+  assert (as_nat h3 x == as_nat h2 x % S.order);
   pop_frame ();
   not is_res_point_at_inf
 
