code/ecdsap256/Hacl.Impl.P256.PointMul.fsti
@@ -38,24 +38,26 @@ val point_mul_g: res:point -> scalar:felem -> Stack unit
     from_mont_point (as_point_nat h1 res) == S.point_mul_g (as_nat h0 scalar))
 
 
-val point_mul_bytes: res:point -> p:point -> scalar:lbuffer uint8 32ul -> Stack unit
+val point_mul_bytes: res:aff_point -> p:point -> scalar:lbuffer uint8 32ul -> Stack uint64
   (requires fun h ->
     live h p /\ live h res /\ live h scalar /\
     disjoint p res /\ disjoint scalar res /\ disjoint p scalar /\
     point_inv h p)
-  (ensures fun h0 _ h1 -> modifies (loc res) h0 h1 /\
-    point_inv h1 res /\
-    as_point_nat h1 res == S.norm_jacob_point
-      (S.point_mul (BSeq.nat_from_bytes_be (as_seq h0 scalar)) (as_point_nat h0 p)))
+  (ensures fun h0 r h1 -> modifies (loc res) h0 h1 /\
+    aff_point_inv h1 res /\
+   (let res_proj = S.point_mul (BSeq.nat_from_bytes_be (as_seq h0 scalar)) (as_point_nat h0 p) in
+    as_aff_point_nat h1 res == S.to_aff_point res_proj /\
+   (if S.is_point_at_inf res_proj then v r = ones_v U64 else v r = 0)))
 
 
-val point_mul_g_bytes: res:point -> scalar:lbuffer uint8 32ul -> Stack unit
+val point_mul_g_bytes: res:aff_point -> scalar:lbuffer uint8 32ul -> Stack uint64
   (requires fun h ->
     live h res /\ live h scalar /\ disjoint res scalar)
-  (ensures fun h0 _ h1 -> modifies (loc res) h0 h1 /\
-    point_inv h1 res /\
-    as_point_nat h1 res == S.norm_jacob_point
-      (S.point_mul_g (BSeq.nat_from_bytes_be (as_seq h0 scalar))))
+  (ensures fun h0 r h1 -> modifies (loc res) h0 h1 /\
+    aff_point_inv h1 res /\
+   (let res_proj = S.point_mul_g (BSeq.nat_from_bytes_be (as_seq h0 scalar)) in
+    as_aff_point_nat h1 res == S.to_aff_point res_proj /\
+   (if S.is_point_at_inf res_proj then v r = ones_v U64 else v r = 0)))
 
 
 val point_mul_double_g: res:point -> scalar1:felem -> scalar2:felem -> p:point -> Stack unit
